compiler/backend/semantics/labSemScript.sml
@@ -354,16 +354,19 @@ val evaluate_def = tDefine "evaluate" `
   \\ decide_tac)
 
 val semantics_def = Define `
-  (semantics s1 (Terminate t io_list) <=>
-     ?k s2.
-       evaluate (s1 with clock := k) = (Halt t,s2) /\
-       (∀e. t = FFI_outcome e ⇒ s2.ffi.final_event = SOME e) ∧
+  (semantics s1 (Terminate outcome io_list) <=>
+     ?k s2 t.
+       evaluate (s1 with clock := k) = (t,s2) /\
+       (case outcome of
+        | FFI_outcome e => (s2.ffi.final_event = SOME e /\ t <> Error)
+        | _ => (s2.ffi.final_event = NONE) /\ (t = Halt outcome)) /\
        s2.ffi.io_events = io_list) /\
   (semantics s1 (Diverge io_trace) <=>
      (!k. ?s2. (evaluate (s1 with clock := k) = (TimeOut,s2)) /\
                s2.ffi.final_event = NONE) /\
-     lprefix_lub (IMAGE (λk. fromList (SND(evaluate (s1 with clock := k))).ffi.io_events) UNIV) io_trace) /\
+     lprefix_lub (IMAGE (\k. fromList
+       (SND (evaluate (s1 with clock := k))).ffi.io_events) UNIV) io_trace) /\
   (semantics s1 Fail <=>
-     ?k s2. (evaluate (s1 with clock := k) = (Error,s2)) ∧ s2.ffi.final_event = NONE)`
+     ?k. FST (evaluate (s1 with clock := k)) = Error)`
 
 val _ = export_theory();
