compiler/backend/semantics/labPropsScript.sml
@@ -124,19 +124,6 @@ val get_byte_set_byte_diff = store_thm("get_byte_set_byte_diff",
   \\ fs [w2w] \\ TRY (match_mp_tac NOT_w2w_bit)
   \\ fs [] \\ decide_tac)
 
-val evaluate_ADD_clock = store_thm("evaluate_ADD_clock",
-  ``!s res r k.
-      evaluate s = (res,r) /\ res <> TimeOut ==>
-      evaluate (s with clock := s.clock + k) = (res,r)``,
-  cheat (* easy *));
-
-val evaluate_final_event_IMP = store_thm("evaluate_final_event_IMP",
-  ``!k s q r.
-      s.ffi.final_event = NONE /\ evaluate s = (q,r) /\
-      r.ffi.final_event = SOME e ==>
-      q = Halt (FFI_outcome e)``,
-  cheat (* easy *));
-
 val evaluate_pres_final_event = store_thm("evaluate_pres_final_event",
   ``!s1.
       (evaluate s1 = (res,s2)) /\ s1.ffi.final_event ≠ NONE ==> s2.ffi = s1.ffi``,
@@ -149,5 +136,9 @@ val evaluate_pres_final_event = store_thm("evaluate_pres_final_event",
   \\ fs [AND_IMP_INTRO]
   \\ res_tac \\ fs [inc_pc_def,dec_clock_def,asm_inst_consts,upd_reg_def]
   \\ rfs [call_FFI_def] \\ fs[] \\ res_tac \\ fs []);
+
+val evaluate_Halt_IMP = store_thm("evaluate_Halt_IMP",
+  ``evaluate s = (Halt x,s2) ==> (x = Success) \/ (x = Resource_limit_hit)``,
+  cheat (* easy *));
 
 val _ = export_theory();
